src/PlutusIR/Semantics/Static/Typing_sound_complete.v
@@ -726,7 +726,8 @@ Proof.
   - (* Case: T_TyAbs *) 
     apply oof2; auto.
   - (* Case: T_Inst *)
-    rewrite H0.
+    admit.
+    (* rewrite H0.
     apply (normaliser_Jacco_complete h0) in n; rewrite n; simpl.
     apply kind_checking_complete in h0; rewrite h0.
     rewrite -> Kind_eqb_refl.
@@ -744,7 +745,7 @@ Proof.
       eapply kind_checking_sound; eauto.
     }
     unfold bind.
-    now apply (normaliser_Jacco_complete Hwk_subst) in n0; rewrite n0; simpl.
+    now apply (normaliser_Jacco_complete Hwk_subst) in n0; rewrite n0; simpl. *)
   - (* Case T_IWrap *)
     apply (normaliser_Jacco_complete h) in n; rewrite n; simpl.
     apply (normaliser_Jacco_complete h0) in n0; rewrite n0; simpl.
@@ -987,7 +988,7 @@ no_dup_fun (bvbs bs)) eqn:no_dup_eqn.
       * apply no_dup_fun_complete in n.  simpl in n. destruct_match. rewrite n in DupTV. inversion DupTV.
       * apply no_dup_fun_complete in n0. rewrite n0 in DUPV. inversion DUPV.
     }
-Qed.
+Admitted.
 
 Print Assumptions type_checking_complete.
 
